cleanup

theories/Strl.v
@@ -2,98 +2,62 @@ Require Import List Uint63 PString Recdef Lia ZifyUint63.
 Open Scope uint63.
 Open Scope pstring.
 
-Definition strl := {x: list string | Forall (fun x => x <> "") x}.
-Fixpoint _slget sl i :=
+Fixpoint slget sl i :=
   match sl with
   | nil => 0
   | a::t =>
       if (i <? length a)
       then get a i
-      else _slget t (i - length a)
+      else slget t (i - length a)
   end.
-Definition slget (sl:strl) i := _slget (proj1_sig sl) i.
-Definition _slcat := @app string.
-Definition slcat (sl1 sl2: strl) : strl.
-Proof.
-  inversion sl1. inversion sl2.
-  exists (x++x0). now apply Forall_app.
-Defined.
-Fixpoint _slsub sl i n :=
+Definition slcat := @app string.
+Fixpoint slsub sl i n :=
   if (n =? 0) then nil else
   match sl with
   | nil => nil
   | a::t =>
       if (i <? length a) then
         let x := sub a i n in
-        x::_slsub t 0 (n - length x)
+        x::slsub t 0 (n - length x)
       else
-        _slsub t (i - length a) n
+        slsub t (i - length a) n
   end.
-Definition slsub (sl: strl) (i n: int) : strl.
-Proof.
-  inversion sl. exists (_slsub x i n).
-  generalize n i. induction x; intros; simpl.
-  - now destruct eqb.
-  - destruct eqb eqn:NE; auto. apply Forall_inv_tail in H.
-    destruct ltb eqn:LT; [| now apply IHx].
-    constructor; [| now apply IHx].
-    intro S; apply (f_equal to_list) in S.
-    rewrite sub_spec in S.
-    apply (f_equal (@List.length _)) in S; cbv [to_list] in S.
-    rewrite length_firstn, length_skipn, length_map, length_seq in S.
-    simpl in S. lia.
-Defined.
-Definition _sllength sl := List.fold_left add (map length sl) 0.
-Definition sllength (sl: strl) := _sllength (proj1_sig sl).
-Definition strl_of_list (sl: list string) : strl.
-Proof.
-  exists (filter (fun x => match compare x "" with | Eq => false | _ => true end) sl).
-  apply Forall_forall. intros. apply filter_In in H as [_ H].
-  intro. now rewrite H0 in H.
-Defined.
-Definition strl_of_string (s: string) : strl.
-Proof.
-  destruct (compare s "") eqn:E. now exists nil.
-  all: exists (s::nil); constructor; try easy; intro; now rewrite H in E.
-Defined.
+Definition sllength sl := List.fold_left add (map length sl) 0.
 Definition slsplice sl i sl2 :=
   slcat (slcat (slsub sl 0 i) sl2) (slsub sl (i + sllength sl2) (sllength sl)).
-Definition list_of_strl (sl: strl) := List.concat (map to_list (proj1_sig sl)).
+Definition list_of_strl sl := List.concat (map to_list sl).
 Notation "'LO'" := list_of_strl.
 Definition slequiv sl1 sl2 := list_of_strl sl1 = list_of_strl sl2.
 Infix "~" := slequiv (at level 10).
 Lemma list_get:
   forall sl i, slget sl i = nth (to_nat i) (LO sl) 0.
 Proof.
-  intros. destruct sl. unfold slget, list_of_strl. simpl. clear f.
-  generalize i. induction x; intro.
+  induction sl; intros; unfold list_of_strl.
     simpl. now destruct (_:nat).
     simpl. destruct ltb eqn:LT.
       rewrite app_nth1. apply get_spec.
       rewrite <-length_spec. lia.
-    rewrite IHx. rewrite app_nth2, <-length_spec. f_equal. lia.
+    rewrite IHsl. rewrite app_nth2, <-length_spec. f_equal. lia.
     rewrite <-length_spec. lia.
 Qed.
 Lemma list_cat:
   forall sl1 sl2, LO (slcat sl1 sl2) = LO sl1 ++ LO sl2.
 Proof.
-  intros. destruct sl1, sl2. unfold slcat, list_of_strl. simpl.
-  now rewrite map_app, concat_app.
+  intros. unfold slcat, list_of_strl. now rewrite map_app, concat_app.
 Qed.
 Lemma list_sub:
   forall sl i n, LO (slsub sl i n) = firstn (to_nat n) (skipn (to_nat i) (LO sl)).
 Proof.
-  intros. destruct sl. unfold slsub, list_of_strl. simpl. clear f.
-  generalize i n. induction x; intros; simpl.
+  unfold list_of_strl. induction sl; intros; simpl.
     destruct eqb; now rewrite skipn_nil, firstn_nil.
     destruct eqb eqn:EQ.
       apply eqb_correct in EQ. now rewrite EQ.
       destruct ltb eqn:LT.
-      - simpl. rewrite IHx, skipn_app, firstn_app.
+      - simpl. rewrite IHsl, skipn_app, firstn_app.
         f_equal. apply sub_spec.
         f_equal. rewrite length_spec_int, sub_spec, length_firstn, length_skipn. lia.
         f_equal. rewrite <-length_spec. lia.
-      - rewrite IHx, skipn_app.
+      - rewrite IHsl, skipn_app.
         f_equal. rewrite (skipn_all2 (to_list a)), app_nil_l.
         f_equal. rewrite <-length_spec. lia.
         rewrite <-length_spec. lia.
@@ -106,10 +70,10 @@ Qed.
 Lemma list_length:
   forall sl, sllength sl = of_nat (List.length (LO sl)).
 Proof.
-  intros. destruct sl. unfold sllength, list_of_strl. simpl. clear f.
-  induction x. easy.
-  unfold _sllength in *. simpl. rewrite fold_add.
-  rewrite IHx. rewrite length_app. rewrite <-length_spec. lia.
+  intros. unfold list_of_strl.
+  induction sl. easy.
+  unfold sllength in *. simpl. rewrite fold_add.
+  rewrite IHsl. rewrite length_app. rewrite <-length_spec. lia.
 Qed.
 (* Lemma list_splice: *)
 (*   forall sl1 i sl2, LO (slsplice sl1 i sl2) = *)
